theories/Subset_Act.v
@@ -1,0 +1,111 @@
+(*
+   Copyright (c) 2024 Nomadic Labs
+   Copyright (c) 2024 Paul Laforgue <paul.laforgue@nomadic-labs.com>
+   Copyright (c) 2024 Léo Stefanesco <leo.stefanesco@mpi-sws.org>
+
+   Permission is hereby granted, free of charge, to any person obtaining a copy
+   of this software and associated documentation files (the "Software"), to deal
+   in the Software without restriction, including without limitation the rights
+   to use, copy, modify, merge, publish, distribute, sublicense, and/or sell
+   copies of the Software, and to permit persons to whom the Software is
+   furnished to do so, subject to the following conditions:
+
+   The above copyright notice and this permission notice shall be included in all
+   copies or substantial portions of the Software.
+
+   THE SOFTWARE IS PROVIDED "AS IS", WITHOUT WARRANTY OF ANY KIND, EXPRESS OR
+   IMPLIED, INCLUDING BUT NOT LIMITED TO THE WARRANTIES OF MERCHANTABILITY,
+   FITNESS FOR A PARTICULAR PURPOSE AND NONINFRINGEMENT. IN NO EVENT SHALL THE
+   AUTHORS OR COPYRIGHT HOLDERS BE LIABLE FOR ANY CLAIM, DAMAGES OR OTHER
+   LIABILITY, WHETHER IN AN ACTION OF CONTRACT, TORT OR OTHERWISE, ARISING FROM,
+   OUT OF OR IN CONNECTION WITH THE SOFTWARE OR THE USE OR OTHER DEALINGS IN THE
+   SOFTWARE.
+*)
+
+Require ssreflect.
+Require Import Coq.Unicode.Utf8.
+Require Import Coq.Lists.List.
+Import ListNotations.
+Require Import Coq.Program.Equality.
+Require Import Coq.Wellfounded.Inverse_Image.
+Require Import Coq.Logic.JMeq.
+Require Import Coq.Program.Wf Setoid.
+Require Import Coq.Program.Equality.
+From Coq.Logic Require Import ProofIrrelevance.
+From stdpp Require Import base countable finite gmap list finite base decidable finite gmap.
+From Must Require Import TransitionSystems.
+
+
+Definition SubSet_Act {A : Type} := A -> Prop.
+
+
+Definition lts_pre_acc_set_of `{Lts P A} (p : P) (μ : A) : Prop := 
+      ¬ lts_stable p (ActExt μ).
+
+Definition lts_acc_set_of `{Lts P A} (p : P) : SubSet_Act := lts_pre_acc_set_of p.
+
+(* Definition Included {A : Type} (B C: A -> Prop) : Prop := 
+    forall μ : A, B μ -> C μ.
+Notation "B ⫅ C" := (Included B C) (at level 20, format "B ⫅ C").
+
+Definition Setminus {A : Type} (B C: A -> Prop) : A -> Prop :=
+    fun μ : A => B μ /\ ~ C μ.
+Notation "B \ C" := (Setminus B C) (at level 20, format "B \ C"). *)
+
+
+Definition Union_of_Act {A :Type} (S : SubSet_Act) (S' : SubSet_Act) (a : A)  : Prop := 
+        S a \/ S' a.
+Definition Intersection_of_Act {A :Type} (S : SubSet_Act) (S' : SubSet_Act) (a : A)  : Prop := 
+        S a /\ S' a.
+Definition Empty_of_Act {A : Type} (x : A) : Prop := False.
+Definition Difference_of_act {A :Type} (S : SubSet_Act) (S' : SubSet_Act) (a : A)  : Prop := 
+        S a /\ (~ (S' a)).
+(* Definition Singleton_of_Act {A : Type} (x : A) : Prop := forall y : A , x = y. *)
+
+(** Instances to use sets notation/properties from stdpp lib *)
+#[global] Instance Union_of_Actions {A : Type} : Union (@SubSet_Act A).
+exact Union_of_Act. Defined.
+#[global] Instance Empty_Actions {A : Type} : Empty (@SubSet_Act A).
+exact Empty_of_Act. Defined.
+#[global] Instance Singleton_of_Actions {A : Type} : Singleton A (@SubSet_Act A).
+intro single_element. exact (fun x : A => single_element = x). Defined.
+#[global] Instance Elements_of {A : Type} : ElemOf A (@SubSet_Act A).
+intro x. intro P. exact (P x). Defined.
+#[global] Instance Intersection_of_Actions {A : Type} : Intersection (@SubSet_Act A).
+exact Intersection_of_Act. Defined.
+#[global] Instance Difference_of_Actions {A : Type} : Difference (@SubSet_Act A).
+exact Difference_of_act. Defined.
+#[global] Instance Top_Actions {A : Type} : Top (@SubSet_Act A).
+intro. exact True. Defined.
+(* #[global] Instance SubsetEq_of_Actions {A : Type} : SubsetEq (@SubSet_Act A).
+intro P. intro Q. exact (forall x : A, P x -> Q x). Defined. *)
+
+
+#[global] Instance SemiSet_of_Actions {A : Type} : SemiSet A (@SubSet_Act A).
+repeat split.
++ intros. intro. exact H.
++ intro. inversion H. reflexivity.
++ intro eq. subst. (* unfold elem_of. unfold singleton. unfold Singleton_of_Actions. 
+    unfold Elements_of. *) reflexivity.
++ intro Hyp. destruct Hyp.
+  ++ left; eauto.
+  ++ right; eauto.
++ intro. destruct H.
+  ++ left; eauto.
+  ++ right; eauto.
+Defined.
+
+#[global] Instance Set_of_Actions {A : Type} : Set_ A (@SubSet_Act A).
+repeat split; try set_solver.
++ destruct H. eauto.
++ destruct H. eauto.
++ destruct H. eauto.
++ destruct H. eauto. Defined.
+
+#[global] Instance TopSet_of_Actions {A : Type} : TopSet A (@SubSet_Act A).
+repeat split ; try set_solver. Defined.
+
+#[global] Instance LeibnizEquiv_Actions {A : Type} : LeibnizEquiv (@SubSet_Act A).
+Admitted.
+
+
